stepPreservesRewind.v
@@ -1,11 +1,5 @@
-Require Export semantics. 
-   
-(*retrieve the stamp number from a heap location*)
-Definition getStamp (x : location * term * lock) :=
-  match x with
-      |(_,_,s) => s
-  end.   
- 
+Require Export noninterference. 
+
 Theorem validInvalidStamp : forall tid S lock,
                               validStamp tid S lock ->
                               invalidStamp tid S lock -> False. 
@@ -13,158 +7,6 @@ Proof.
   intros tid S lock H H0.
   inv H; inv H0; auto. omega.
 Qed.
-
-Inductive locked (tid : nat) : lock -> Prop :=
-|acquired : forall oldV v, locked tid (Locked tid oldV v). 
- 
-Theorem validateNotIn : 
-  forall tid l v b v'' lock''' rv wv e0 L H lock' chkpnt HI HV,
-    Log.notIn l b L -> H l = Some(v'', lock''') -> validStamp tid rv lock''' -> 
-    @validate tid rv wv e0 b L (update H l v lock') 
-              (commit chkpnt HI HV) ->
-    exists HV', @validate tid rv wv e0 b L H (commit chkpnt (update HI l v'' lock''') HV').
-Proof.   
-  intros tid l v b v'' lock''' rv wv e0 L H lock' chkpnt HI HV H0 H1 HV2 H3.
-  remember (update H l v lock'). remember (commit chkpnt HI HV).
-  genDeps{{chkpnt; HI; HV; H; l; v; lock'; lock'''}}.
-  induction H3; intros; try solve[inv Heqv0].
-  {inv Heqv0. subst. exists H1. rewrite updateUpdate.
-   rewrite updateIdempotent. constructor. eassumption. }
-  {inv Heqv0. dependent destruction H2. eapply IHvalidate in H2; eauto. 
-   invertHyp. unfold lookup in H0. unfold update in H0. 
-   destruct (Nat.eq_dec l0 l). 
-   {subst. econstructor. econstructor; eauto. } 
-   {econstructor. econstructor; eauto. }
-  }
-  {inv Heqv0. dependent destruction H2. eapply IHvalidate in H2; eauto. 
-   invertHyp. unfold lookup in H0. unfold update in H0. 
-   destruct (Nat.eq_dec l0 l). 
-   {subst. econstructor. econstructor; eauto. } 
-   {econstructor. econstructor; eauto. }
-  }
-  {inv Heqv0. dependent destruction H1. 
-   eapply IHvalidate in H1; eauto. invertHyp. econstructor. 
-   rewrite updatecomm; auto. econstructor; eauto. unfold lookup in H0. 
-   unfold update in H0. destruct (Nat.eq_dec l0 l). contradiction. 
-   eassumption. }
-Qed. 
-
-Theorem validateIn :  
-  forall tid l v v'' rv wv e0 L H lock' chkpnt HI HV,
-    Log.In l L -> H l = Some(v'', lock') -> 
-    @validate tid rv wv e0 true L (update H l v lock') 
-              (commit chkpnt HI HV) ->
-    exists HV', @validate tid rv wv e0 true L H (commit chkpnt HI HV').
-Proof.
-  intros. dependent induction H2.
-  {dependent destruction H0. eapply IHvalidate in H0; eauto. 
-   invertHyp. unfold lookup in H4. unfold update in H4.
-   destruct (Nat.eq_dec l l0).
-   {subst. inv H4. econstructor. econstructor; eauto. }
-   {econstructor. econstructor; eauto. }
-  }
-  {dependent destruction H0.
-   {unfold lookup in H3. unfold update in H3.
-    destruct (Nat.eq_dec l0 l0). Focus 2. exfalso; eauto.
-    inv H3. eapply validateNotIn in H0; eauto. invertHyp.
-    erewrite <- updateUpdate. econstructor. econstructor; eauto. constructor. }
-   {eapply IHvalidate in H1; eauto. invertHyp. econstructor.
-    econstructor; eauto. unfold lookup in H3. unfold update in H3.
-    destruct (Nat.eq_dec l l0). contradiction. eassumption. }
-  }
-Qed. 
-
-Theorem validateAcquiredLock : forall tid l v v' b rv wv e0 L L' H lock lock' chkpnt HI HV,
-    lookup H l = Some(v', lock) ->
-    acquireLock l v' tid rv L lock lock' L' -> 
-    @validate tid rv wv e0 true L' (update H l v lock') (commit chkpnt HI HV) ->
-    exists HV', @validate tid rv wv e0 b L H (commit chkpnt HI HV').
-Proof.
-  intros tid l v v' b rv wv e0 L L' H lock lock' chkpnt HI HV H0 H1 H2.
-  dependent destruction H1. 
-  {eapply validateIn in H1; eauto. }
-  {dependent destruction H3. unfold update in H4. unfold lookup in H4. 
-   destruct (Nat.eq_dec l l). inv H4. 
-   eapply validateNotIn in H5; eauto. 
-   constructor. omega. exfalso; auto. }
-Qed. 
-
-Theorem abortNotIn : 
-  forall tid l v b v'' lock''' rv wv e0 L H lock' chkpnt HI,
-    Log.notIn l b L -> H l = Some(v'', lock''') -> validStamp tid rv lock''' ->
-    locked tid lock' ->
-    @validate tid rv wv e0 b L (update H l v lock') (abort chkpnt HI) ->
-    @validate tid rv wv e0 b L H (abort chkpnt (update HI l v'' lock''')).
-Proof.
-  intros. remember (update H l v lock'). remember (abort chkpnt HI).
-  genDeps{{chkpnt; HI; H; l; v; lock'}}.
-  induction H4; intros; try solve[inv Heqv0]. 
-  {inv Heqv0. dependent destruction H5. eapply validateNotIn in H5; eauto. 
-   invertHyp. unfold lookup in H0. unfold update in H0.
-   destruct (Nat.eq_dec l0 l).
-   {subst. inv H0. inv H3. inv H1. exfalso; auto. }
-   {econstructor; eauto. }
-  }
-  {inv Heqv0. dependent destruction H5. eapply validateNotIn in H5; eauto. 
-   invertHyp. unfold lookup in H0. unfold update in H0.
-   destruct (Nat.eq_dec l0 l).
-   {subst. inv H0. inv H3. inv H1. exfalso; auto. }
-   {econstructor; eauto. }
-  }
-  {dependent destruction H0.
-   {dependent destruction H1. eapply IHvalidate in H1; eauto.
-    subst. inv Heqv0. eapply readPropAbort; eauto. constructor. }
-   {inv Heqv0. dependent destruction H1. eapply IHvalidate in H1; eauto.
-    eapply readPropAbort; eauto. constructor. }
-  }
-  {dependent destruction H1. inv Heqv0. eapply IHvalidate in H5; eauto.
-   unfold lookup in H0. unfold update in H0. destruct (Nat.eq_dec l0 l).
-   contradiction. rewrite updatecomm; auto. eapply writePropAbort. auto.
-   eauto. }
-Qed.
-
-Theorem abortIn :  
-  forall tid l v v'' rv wv e0 L H lock' chkpnt HI,
-    Log.In l L -> H l = Some(v'', lock') -> 
-    @validate tid rv wv e0 true L (update H l v lock') 
-              (abort chkpnt HI) ->
-    @validate tid rv wv e0 true L H (abort chkpnt HI).
-Proof.
-  intros. dependent induction H2.
-  {dependent destruction H0. eapply validateIn in H0; eauto.
-   invertHyp. unfold lookup in H4. unfold update in H4. destruct (Nat.eq_dec l l0).
-   {subst. inv H4. econstructor; eauto. }
-   {econstructor; eauto. }
-  }
-  {dependent destruction H3. dependent destruction H0. eapply IHvalidate in H0; eauto.
-   eapply readPropAbort; eauto. constructor. }
-  {dependent destruction H0.
-   {unfold lookup in H3. unfold update in H3. destruct (Nat.eq_dec l0 l0).
-    {inv H3. eapply abortNotIn in H0; eauto. erewrite <- updateUpdate.
-     eapply writePropAbort; eauto. constructor. constructor. }
-    {exfalso; auto. }
-   }
-   {eapply IHvalidate in H1; eauto. eapply writePropAbort; eauto.
-    unfold lookup in H3. unfold update in H3. destruct (Nat.eq_dec l l0).
-    contradiction. eauto. }
-  }
-Qed. 
-
-Theorem abortAcquiredLock : forall tid l v v' b rv wv e0 L L' H lock lock' chkpnt HI,
-    lookup H l = Some(v', lock) ->
-    acquireLock l v' tid rv L lock lock' L' -> 
-    @validate tid rv wv e0 true L' (update H l v lock') (abort chkpnt HI) ->
-    @validate tid rv wv e0 b L H (abort chkpnt HI).
-Proof.
-  intros. dependent destruction H1. 
-  {eapply abortIn in H2; eauto. }
-  {dependent destruction H3. dependent destruction H5.
-   unfold update in H5. unfold lookup in H5. 
-   destruct (Nat.eq_dec l l). inv H5. 
-   eapply abortNotIn in H2; eauto. constructor. auto. constructor. 
-   exfalso; auto. }
-Qed. 
-
    
 Theorem rewindNewerStamp : forall S C H1 H2 b1 b2 tid e0 L1 L2 t1 t2 HI HV chkpnt,
                              rewind H1 (txThread b1 tid S e0 L1 t1)
@@ -185,7 +27,7 @@ Proof.
      eapply r_readNoChkpnt; eauto. transEq. invertEq.
      inv H7; econstructor; eauto. omega. }
    {(*r_readStepInvalid*)
-     dependent destruction H6. transEq. invertEq. exfalso.
+     dependent destruction H7. transEq. invertEq. exfalso.
      eapply validInvalidStamp; eauto. }
    { (*r_writeLocked*) 
      copy H4. eapply validateAcquiredLock in H4; eauto. invertHyp.
@@ -199,65 +41,6 @@ Proof.
   }
 Qed. 
 
-Theorem notInUpdate : forall H l v lock l',
-    (update H l v lock) l' = None ->
-    H l' = None. 
-Proof.
-  intros. unfold update in H0. destruct (Nat.eq_dec l l').
-  {inv H0. }
-  {assumption.  }
-Qed.
-
-(* `Nat.eq_dec l l'` == {l = l'} + {l <> l'}
- * is of type `sumbool`
- *)
-
-Ltac heapUnfold := unfold lookup; unfold update.
-
-Theorem rewindAllocSingle : forall tid H H' b1 b2 S e0 L l v L' e e',
-    H' l = None ->
-    rewind H (txThread b1 tid S e0 L e) H' (txThread b2 tid S e0 L' e') ->
-    exists H'', rewind H'' (txThread b1 tid S e0 L e) (update H' l v (Unlocked 0)) (txThread b2 tid S e0 L' e').
-Proof.
-  intros tid H H' b1 b2 S e0 L l v L' e e' H0 H1. genDeps{{l; v}}. 
-  induction H1; intros.
-  {repeat econstructor. }
-  {inv H0.
-   {copy H2. eapply IHrewind in H2. invertHyp. exists x. econstructor; eauto.
-    econstructor; eauto. destruct (eq_nat_dec l l0).
-    {subst. unfold lookup in H5. transEq. invertEq. }
-    {unfold lookup. unfold update. simplEq l l0. auto. }
-   }
-   {copy H2. eapply IHrewind in H0. invertHyp. exists x. econstructor. eauto.
-    econstructor; eauto. heapUnfold. destruct (Nat.eq_dec l l0); auto. 
-    subst. unfold lookup in *. transEq. invertEq. }
-   {copy H2. eapply IHrewind in H2. invertHyp. exists x. econstructor.
-    eauto. eapply r_readStepInvalid; eauto. destruct (Nat.eq_dec l l0); eauto. 
-    {unfold lookup in H5. subst. transEq. invertEq. }
-    {unfold lookup. unfold update. simplEq l l0. eauto. }
-   }
-   {copy H2. eapply notInUpdate in H2; eauto. eapply IHrewind in H2. invertHyp.
-    exists x. econstructor; eauto. destruct (Nat.eq_dec l l0).
-    {subst. unfold update in H0. destruct (Nat.eq_dec l0 l0). invertEq.
-     exfalso. apply n. auto. }
-    {rewrite <- updatecomm; auto. econstructor; eauto. heapUnfold. simplEq l l0.
-     auto. }
-   }
-   {eapply IHrewind in H2. invertHyp. exists x. econstructor; eauto. eapply r_atomicIdemStep; eauto. }
-   {eapply IHrewind in H2. invertHyp. exists x. econstructor; eauto. eapply r_betaStep; eauto. }
-  }
-Qed. 
-  
-Theorem rewindAlloc : forall C H T l v,
-    H l = None -> 
-    poolRewind C H T -> poolRewind C (update H l v (Unlocked 0)) T. 
-Proof.
-  intros C H T l v H0 H1. genDeps{{l; v}}. induction H1; intros.
-  {constructor. }
-  {eapply rewindAllocSingle in H0; eauto.  invertHyp. econstructor; eauto. }
-  {econstructor; eauto. }
-Qed. 
-   
 Theorem poolRewindNewerStamp : forall C C' H T,
     poolRewind C H T -> C' > C -> poolRewind C' H T. 
 Proof.
@@ -266,8 +49,7 @@ Proof.
   {econstructor; eauto. omega. }
   {econstructor; eauto. }
 Qed. 
-
-   
+    
 Theorem f_rewindNoninterference : forall C H C' H' T T' T2,
     f_step C H T C' H' T' -> poolRewind C H T2 ->
     poolRewind C' H' T2.
@@ -275,16 +57,12 @@ Proof.
   intros C H C' H' T T' T2 H0 H1. generalize dependent T2.
   induction H0; intros; eauto. 
   {(*if someone else aborts, then we can still rewind*)
-    inv H0.
-
-    
-
-   admit. }
+    inv H0. eapply abortRewindNI; eauto. }
   {inv H0; auto.  
    {admit. }
   }
   {eapply rewindAlloc; auto. }
-  {admit. }
+  {eapply commitRewindNI; eauto. }
   {eapply poolRewindNewerStamp; eauto. }
   {eapply poolRewindNewerStamp; eauto. }
 Admitted. 
@@ -295,12 +73,12 @@ Theorem p_rewindNoninterference : forall C H C' H' T T' T2,
 Proof.
   intros C H C' H' T T' T2 H0 H1. generalize dependent T2.
   induction H0; intros; eauto. 
-  {inv H0. admit. }
+  {inv H0. eapply abortRewindNI; eauto. }
   {inv H0; auto.  
    {admit. }
   }
   {eapply rewindAlloc; auto. }
-  {admit. }
+  {eapply commitRewindNI; eauto. }
   {eapply poolRewindNewerStamp; eauto. }
   {eapply poolRewindNewerStamp; eauto. }
 Admitted.     
@@ -357,7 +135,7 @@ Proof.
     eapply rewindNewerStamp with (C := C); eauto. apply decomposeEq in H1.
     subst. assumption. }
    {dependent destruction H6. eapply IHrewind; eauto. }
-   {dependent destruction H6. transEq. invertEq. exfalso.
+   {dependent destruction H7. transEq. invertEq. exfalso.
     eapply validInvalidStamp; eauto. }
    {(*validWrite*)
      eapply validateAcquiredLock in H2; eauto. invertHyp. 
@@ -399,20 +177,14 @@ Proof.
     (*readPropAbort: this read is valid, but an earlier one is out of date, use IH*)
     {dependent destruction H6. eapply IHrewind; eauto. }
    }
-   {dependent destruction H5.   (*r_readStepInvalid*)
+   {dependent destruction H6.   (*r_readStepInvalid*)
     {(*invalidRead: this read is invalid, but we don't have a checkpoint*)
       transEq. invertEq. eapply commitRewind; eauto. }
-    {dependent destruction H6. eauto. }
+    {dependent destruction H7. eauto. }
    }
    {eapply abortAcquiredLock in H5; eauto. }
   }
 Qed.
-
-Definition invalidHeap res :=
-  match res with
-  |commit _ H _ => H
-  |abort _ H => H
-  end. 
 
 Theorem validateRewindHeapEq : forall res b H H'' tid S  L'' e' e0 C,
     @validate tid S C e0 b L'' H res ->
@@ -433,10 +205,10 @@ Proof.
     {eapply IHrewind in H7; eauto. }
     {dependent destruction H6. eapply IHrewind in H5; eauto. }
    }
-   {dependent destruction H5.
+   {dependent destruction H6.
     {transEq. invertEq. exfalso. eapply validInvalidStamp; eauto. }
-    {transEq. invertEq. eapply IHrewind in H7; eauto. }
-    {dependent destruction H6. eapply IHrewind in H5; eauto. }
+    {transEq. invertEq. eapply IHrewind in H8; eauto. }
+    {dependent destruction H7. eapply IHrewind in H6; eauto. }
    }
    {destruct res.
     {eapply validateAcquiredLock in H4; eauto. invertHyp.
